theories/examples/contiguous.v
@@ -707,3 +707,35 @@ Section Contiguous.
 End Contiguous.
 
 Opaque contiguous.
+
+Definition isCorrectPC_range p g b e a0 an :=
+  ∀ ai, (a0 <= ai)%a ∧ (ai < an)%a → isCorrectPC (inr (p, g, b, e, ai)).
+
+Lemma isCorrectPC_inrange p g b (e a0 an a: Addr) :
+  isCorrectPC_range p g b e a0 an →
+  (a0 <= a < an)%Z →
+  isCorrectPC (inr (p, g, b, e, a)).
+Proof.
+  unfold isCorrectPC_range. move=> /(_ a) HH ?. apply HH. eauto.
+Qed.
+
+Lemma isCorrectPC_contiguous_range p g b e a0 an a l :
+  isCorrectPC_range p g b e a0 an →
+  contiguous_between l a0 an →
+  a ∈ l →
+  isCorrectPC (inr (p, g, b, e, a)).
+Proof.
+  intros Hr Hc Hin.
+  eapply isCorrectPC_inrange; eauto.
+  eapply contiguous_between_middle_bounds'; eauto.
+Qed.
+
+Lemma isCorrectPC_range_perm p g b e a0 an :
+  isCorrectPC_range p g b e a0 an →
+  (a0 < an)%a →
+  p = RX ∨ p = RWX ∨ p = RWLX.
+Proof.
+  intros Hr H0n.
+  assert (isCorrectPC (inr (p, g, b, e, a0))) as HH by (apply Hr; solve_addr).
+  inversion HH; auto.
+Qed.
